added more n-ary facts and structures

src/PredCalc/SequentialSubst.v
@@ -1,35 +1,17 @@
 From Equations Require Import Equations.
 From Stdlib Require Import Lia.
 From Stdlib Require Import Lists.List.
-From stdpp Require Import base list_monad.
+From stdpp Require Import base list_monad sets.
 From MRC Require Import Prelude.
 From MRC Require Import Stdppp.
 From MRC Require Import Model.
+From MRC Require Import SeqNotation.
 From MRC Require Import PredCalc.Basic.
+From MRC Require Import PredCalc.Equiv.
 From MRC Require Import PredCalc.SemanticFacts.
+From MRC Require Import PredCalc.EquivLemmas.
 
 (* TODO: move it *)
-Definition of_same_length_rest {A B} {x1 : A} {l1 : list A} {x2 : B} {l2 : list B}
-                              (H : OfSameLength (x1::l1) (x2::l2)) : OfSameLength l1 l2.
-Proof. unfold OfSameLength in *. simpl in H. lia. Defined.
-
-Instance of_same_length_rev {A B} {l1 : list A} {l2 : list B}
-                              `{OfSameLength _ _ l1 l2} : OfSameLength (rev l1) (rev l2).
-Proof. unfold OfSameLength in *. do 2 rewrite length_rev. assumption. Defined.
-
-Definition of_same_length_rect {A B X Y} (f_nil : X → Y) (f_cons : (X → Y) → A → B → X → Y)
-  (x : X)
-  (l1 : list A) (l2 : list B)
-  `{OfSameLength _ _ l1 l2} : Y.
-Proof.
-  generalize dependent x. generalize dependent l2.
-  induction l1 as [|x1 l1' rec], l2 as [|x2 l2']; intros H.
-  - exact f_nil.
-  - inversion H.
-  - inversion H.
-  - apply of_same_length_rest in H. specialize (rec _ H). exact (f_cons rec x1 x2).
-Defined.
-
 Open Scope refiney_scope.
 
 Section sequential_subst.
@@ -48,20 +30,240 @@ Section sequential_subst.
   Implicit Types ts : list term.
   Implicit Types vs : list value.
 
+  (** Equivalene of lists of terms **)
+  Global Instance term_list_equiv : Equiv (list term) :=
+    λ ts1 ts2, length ts1 = length ts2 ∧ Forall2 (≡@{term}) ts1 ts2.
+
+  Global Instance term_list_equiv_refl : Reflexive term_list_equiv.
+  Proof with auto.
+    intros ts. induction ts; hnf... split... apply Forall2_cons. split... apply IHts.
+  Qed.
+
+  Global Instance term_list_equiv_sym : Symmetric term_list_equiv.
+  Proof with auto.
+    intros ts1. induction ts1 as [|t1 ts1 IH]; intros ts2 [H1 H2]; hnf.
+    - simpl in H1. symmetry in H1. apply length_zero_iff_nil in H1. subst ts2...
+    - simpl in H1. symmetry in H1. apply length_nonzero_iff_cons in H1 as (t2&ts2'&?&?).
+      subst ts2. rename ts2' into ts2. split.
+      + do 2 rewrite length_cons...
+      + apply Forall2_cons. apply Forall2_cons in H2 as []. split... apply IH.
+        split...
+  Qed.
+
+  Global Instance term_list_equiv_trans : Transitive term_list_equiv.
+  Proof with auto.
+    intros ts1. induction ts1 as [|t1 ts1 IH]; intros ts2 ts3 [] [].
+    - simpl in H. rewrite <- H in H1. symmetry in H, H1.
+      apply length_zero_iff_nil in H, H1. subst. split...
+    - simpl in H. rewrite <- H in H1. symmetry in H, H1.
+      apply length_nonzero_iff_cons in H as (t2&ts2'&?&?). subst ts2. rename ts2' into ts2.
+      apply length_nonzero_iff_cons in H1 as (t3&ts3'&?&?). subst ts3. rename ts3' into ts3.
+      split.
+      + do 2 rewrite length_cons...
+      + rewrite Forall2_cons in *. destruct H0 as [], H2 as []. split.
+        * trans t2...
+        * forward (IH ts2 ts3) by (split; auto). forward IH by (split; auto; lia).
+          apply IH.
+  Qed.
+
+  Global Instance term_list_equiv_equiv : Equivalence term_list_equiv.
+  Proof.
+    split; [exact term_list_equiv_refl | exact term_list_equiv_sym |
+             exact term_list_equiv_trans].
+  Qed.
+
+  Global Instance cons_proper_term_list_equiv :
+    Proper ((≡@{term}) ==> term_list_equiv ==> term_list_equiv) cons.
+  Proof.
+    intros t1 t2 Ht ts1 ts2 Hts. unfold term_list_equiv in *.
+    do 2 rewrite length_cons. rewrite Forall2_cons. naive_solver.
+  Qed.
+
+  Lemma term_list_equiv_cons_l t1 ts1 ts2 :
+    t1 :: ts1 ≡ ts2 ↔ ∃ t2 ts2', ts2 = t2 :: ts2' ∧ t1 ≡ t2 ∧ ts1 ≡ ts2'.
+  Proof with auto.
+    split.
+    - intros []. symmetry in H. rewrite length_cons in H.
+      apply length_nonzero_iff_cons in H as (t2&ts2'&?&?). subst ts2. rename ts2' into ts2.
+      exists t2, ts2. apply Forall2_cons in H0 as []. split_and!... split...
+    - intros (t2&ts2'&?&?&?). rewrite H. apply cons_proper_term_list_equiv...
+  Qed.
+
+  Lemma term_list_equiv_cons_r ts1 t2 ts2 :
+    ts1 ≡ t2 :: ts2 ↔ ∃ t1 ts1', ts1 = t1 :: ts1' ∧ t1 ≡ t2 ∧ ts1' ≡ ts2.
+  Proof with auto.
+    split.
+    - intros. symmetry in H. apply term_list_equiv_cons_l in H as (t1&ts1'&?&?&?).
+      exists t1, ts1'. split_and!...
+    - intros (t1&ts1'&?&?&?). rewrite H. apply cons_proper_term_list_equiv...
+  Qed.
+
+  Lemma term_list_equiv_nil_l ts :
+    [] ≡ ts ↔ ts = [].
+  Proof with auto.
+    unfold equiv, term_list_equiv. simpl. split.
+    - intros []. symmetry in H. apply length_zero_iff_nil in H. subst...
+    - intros ->. simpl...
+  Qed.
+
+  Lemma term_list_equiv_nil_r ts :
+    ts ≡ [] ↔ ts = [].
+  Proof with auto.
+    unfold equiv, term_list_equiv. simpl. split.
+    - intros []. apply length_zero_iff_nil in H. subst...
+    - intros ->. simpl...
+  Qed.
+
+  Global Instance app_proper_term_list_equiv :
+    Proper ((term_list_equiv) ==> term_list_equiv ==> term_list_equiv) app.
+  Proof with auto.
+    intros ts1 ts3 H13 ts2 ts4 H24. generalize dependent ts3.
+    induction ts1 as [|t1 ts1 IH]; intros ts3 H13.
+    - simpl. apply term_list_equiv_nil_l in H13. subst. simpl...
+    - simpl. apply term_list_equiv_cons_l in H13 as (t3&ts3'&->&?&?). rename ts3' into ts3.
+      simpl. f_equiv...
+  Qed.
+
+  Lemma term_list_equiv_cons_inv t1 ts1 t2 ts2 :
+    t1 :: ts1 ≡ t2 :: ts2 → t1 ≡ t2 ∧ ts1 ≡ ts2.
+  Proof with auto.
+    intros []. do 2 rewrite length_cons in H. apply Forall2_cons in H0 as [].
+    split... split...
+  Qed.
+
+  (** Sequential substitution **)
   Definition seq_subst A xs ts `{OfSameLength _ _ xs ts} : formula :=
     of_same_length_rect (λ A, A) (λ rec x t B, <! $(rec B)[x \ t] !>) A xs ts.
 
-  Definition teval_var_term_list σ xs vs :=
-    OfSameLength xs vs ∧ Forall2 (λ x v, teval σ x v) xs vs.
+  Local Notation "A [; xs \ ts ;]" := (seq_subst A xs ts)
+                              (in custom formula at level 74, left associativity,
+                                xs custom seq_notation,
+                                ts custom term_seq_notation) : refiney_scope.
 
-  Lemma teval_var_list_total σ xs :
-    ∃ vs, teval_var_term_list σ xs vs.
+  Lemma seq_subst_cons A x t xs ts
+    {Hl1 : OfSameLength xs ts} {Hl2 : OfSameLength (x :: xs) (t :: ts)} :
+    @seq_subst A (x :: xs) (t :: ts) Hl2 ≡ <! $(@seq_subst A xs ts Hl1)[x \ t] !>.
   Proof with auto.
-    induction xs as [|x xs IH].
-    - exists []. split... apply of_same_length_nil.
-    - destruct IH as [vs [H1 H2]]. pose proof (teval_total σ x) as [v Hv].
-      exists (v :: vs). split... apply of_same_length_cons.
+    unfold seq_subst. simpl. f_equiv. f_equiv. apply eq_pi. solve_decision.
   Qed.
+
+  Lemma seq_subst_app A xs1 ts1 xs2 ts2
+    {Hl1 :OfSameLength xs1 ts1}
+    {Hl2 : OfSameLength xs2 ts2}
+    {Hl3 : OfSameLength (xs1 ++ xs2) (ts1 ++ ts2)} :
+    @seq_subst A (xs1 ++ xs2) (ts1 ++ ts2) Hl3 ≡
+    @seq_subst (@seq_subst A xs2 ts2 Hl2) xs1 ts1 Hl1.
+  Proof with auto.
+    generalize dependent ts1. generalize dependent xs2. generalize dependent ts2.
+    induction xs1; intros.
+    - inversion Hl1. symmetry in H0. apply length_zero_iff_nil in H0. subst.
+      simpl. f_equiv. apply eq_pi. solve_decision.
+    - inversion Hl1. symmetry in H0. apply length_nonzero_iff_cons in H0 as (t1&ts1'&?&?).
+      subst ts1. rename ts1' into ts1. simpl. intros σ.
+      pose proof (teval_total σ t1) as [v1 Hv1]. rewrite feval_subst with (v:=v1)...
+      rewrite feval_subst with (v:=v1)... specialize (IHxs1 ts2 xs2).
+      assert (OfSameLength xs2 ts2).
+      { unfold OfSameLength. unfold OfSameLength in Hl3. simpl in Hl3.
+        do 2 rewrite length_app in Hl3. rewrite H0 in Hl3. lia. }
+      assert (OfSameLength xs1 ts1) by (symmetry in H0; apply H0).
+      assert (OfSameLength (xs1 ++ xs2) (ts1 ++ ts2)).
+      { apply of_same_length_app. }
+      specialize (IHxs1 H ts1 H1 H2 (<[a:=v1]> σ)).
+      eapply eq_rect.
+      + symmetry. eapply eq_rect.
+        * symmetry. exact IHxs1.
+        * f_equiv. f_equiv. apply eq_pi. solve_decision.
+      + f_equiv. f_equal.
+        * f_equiv. apply eq_pi. solve_decision.
+        * apply eq_pi. solve_decision.
+  Qed.
+
+  Lemma seq_subst_snoc A x t xs ts
+    {Hl1 : OfSameLength xs ts}
+    {Hl2 : OfSameLength (xs ++ [x]) (ts ++ [t])} :
+    @seq_subst A (xs ++ [x]) (ts ++ [t]) Hl2 ≡ @seq_subst (<! A [x \ t] !>) xs ts Hl1.
+  Proof with auto.
+    simpl. rewrite (seq_subst_app A xs ts [x] [t]). f_equiv.
+  Qed.
+
+  (**  [seq_subst] respects [fequiv] and [fent] when [ts] are equivalent under
+       [term_list_equiv].
+       The important part about the following instances is that they discard [OfSameLength]
+       instances. This can be done since equality proofs are proof irrelevant *)
+  Global Instance seq_subst_proper : Proper ((≡@{formula}) ==>
+        respectful_hetero (list variable) (list variable)
+        (λ xs, ∀ ts, OfSameLength xs ts → formula)
+        (λ xs, ∀ ts, OfSameLength xs ts → formula)
+        (=)
+        (λ xs xs', (respectful_hetero (list term) (list term)
+                      (λ ts, OfSameLength xs ts → formula)
+                      (λ ts, OfSameLength xs' ts → formula)
+                      (term_list_equiv)
+                      (λ ts ts', (respectful_hetero (OfSameLength xs ts) (OfSameLength xs' ts')
+                                    (λ _, formula)
+                                    (λ _, formula)
+                                    (λ _ _, True)
+                                    (λ _ _, (≡@{formula}))))))) seq_subst.
+  Proof with auto.
+    intros A B Hequiv xs ? <- ts1 ts2 Hts Hl1 Hl2 _.
+    generalize dependent ts2. generalize dependent ts1.
+    induction xs as [|x xs IH]; intros.
+    - inversion Hl1. inversion Hl2. symmetry in H0, H1. apply length_zero_iff_nil in H0, H1.
+      subst. simpl...
+    - inversion Hl1. inversion Hl2. symmetry in H0, H1.
+      apply length_nonzero_iff_cons in H0 as (t1&ts1'&?&?). subst ts1. rename ts1' into ts1.
+      apply length_nonzero_iff_cons in H1 as (t2&ts2'&?&?). subst ts2. rename ts2' into ts2.
+      apply of_same_length_rest in Hl1 as Hl1'. apply of_same_length_rest in Hl2 as Hl2'.
+      do 2 rewrite seq_subst_cons. apply term_list_equiv_cons_inv in Hts as [].
+       f_equiv...
+      Unshelve.
+      + exact Hl1'.
+      + exact Hl2'.
+  Qed.
+
+  Global Instance seq_subst_proper_fent : Proper ((⇛@{M}) ==>
+        respectful_hetero (list variable) (list variable)
+        (λ xs, ∀ ts, OfSameLength xs ts → formula)
+        (λ xs, ∀ ts, OfSameLength xs ts → formula)
+        (=)
+        (λ xs xs', (respectful_hetero (list term) (list term)
+                      (λ ts, OfSameLength xs ts → formula)
+                      (λ ts, OfSameLength xs' ts → formula)
+                      (term_list_equiv)
+                      (λ ts ts', (respectful_hetero (OfSameLength xs ts) (OfSameLength xs' ts')
+                                    (λ _, formula)
+                                    (λ _, formula)
+                                    (λ _ _, True)
+                                    (λ _ _, (⇛@{M}))))))) seq_subst.
+  Proof with auto.
+    intros A B Hequiv xs ? <- ts1 ts2 Hts Hl1 Hl2 _.
+    generalize dependent ts2. generalize dependent ts1.
+    induction xs as [|x xs IH]; intros.
+    - inversion Hl1. inversion Hl2. symmetry in H0, H1. apply length_zero_iff_nil in H0, H1.
+      subst. simpl...
+    - inversion Hl1. inversion Hl2. symmetry in H0, H1.
+      apply length_nonzero_iff_cons in H0 as (t1&ts1'&?&?). subst ts1. rename ts1' into ts1.
+      apply length_nonzero_iff_cons in H1 as (t2&ts2'&?&?). subst ts2. rename ts2' into ts2.
+      apply of_same_length_rest in Hl1 as Hl1'. apply of_same_length_rest in Hl2 as Hl2'.
+      do 2 rewrite seq_subst_cons. apply term_list_equiv_cons_inv in Hts as [].
+       f_equiv...
+      Unshelve.
+      + exact Hl1'.
+      + exact Hl2'.
+  Qed.
+
+  (** Expanding teval_total to a list of terms **)
+  (* Definition teval_var_term_list σ xs vs := *)
+  (*   OfSameLength xs vs ∧ Forall2 (λ x v, teval σ x v) xs vs. *)
+
+  (* Lemma teval_var_list_total σ xs : *)
+  (*   ∃ vs, teval_var_term_list σ xs vs. *)
+  (* Proof with auto. *)
+  (*   induction xs as [|x xs IH]. *)
+  (*   - exists []. split... apply of_same_length_nil. *)
+  (*   - destruct IH as [vs [H1 H2]]. pose proof (teval_total σ x) as [v Hv]. *)
+  (*     exists (v :: vs). split... apply of_same_length_cons. *)
+  (* Qed. *)
 
   Lemma simpl_feval_forall_list σ xs A :
     feval σ <! ∀* xs, A !> ↔
@@ -87,17 +289,63 @@ Section sequential_subst.
         apply eq_pi. solve_decision.
   Qed.
 
+
+  (** Expanding equality atomic formulas to list of  **)
+
   Definition AT_TermListEq ts1 ts2 `{OfSameLength _ _ ts1 ts2} : formula :=
     of_same_length_rect (λ A, A) (λ rec t1 t2 B, <! ⌜t1 = t2⌝ ∧ $(rec B) !>) <! true !> ts1 ts2.
 
-  Lemma f_forall_list_one_point xs ts A `{OfSameLength _ _ xs ts} :
-      (list_to_set xs) ∩ ⋃ (term_fvars <$> ts) = ∅ →
-      <! ∀* xs, $(AT_TermListEq (TVar <$> xs) ts) ⇒ A !> ≡ seq_subst A xs ts.
+  Lemma term_list_eq_cons t1 t2 ts1 ts2
+    {H1 : OfSameLength ts1 ts2}
+    {H2 : OfSameLength (t1 :: ts1) (t2 :: ts2)} :
+    AT_TermListEq (t1 :: ts1) (t2 :: ts2) ≡ <! ⌜t1 = t2⌝ ∧ $(AT_TermListEq ts1 ts2) !>.
+  Proof. unfold AT_TermListEq. simpl. f_equiv. f_equiv. apply eq_pi. solve_decision. Qed.
+
+  (* Lemma f_forall_list_unused x A : *)
+  (*   x  *)
+  (*   x ∉ formula_fvars A → *)
+  (*   <! ∀ x, A !> ≡ A. *)
+  (* Proof with auto. *)
+  (*   unfold FForall. intros. rewrite fexists_unused... intros σ. *)
+  (*   simp feval. rewrite feval_stable... *)
+  (* Qed. *)
+
+  Lemma fvars_forall_list xs A :
+    formula_fvars <! ∀* xs, A !> = formula_fvars A ∖ list_to_set xs.
+  Proof with auto. induction xs; simpl; set_solver. Qed.
+
+  (* A.65 *)
+  Lemma f_forall_list_and xs A B :
+    <! ∀* xs, A ∧ B !> ≡ <! (∀* xs, A) ∧ (∀* xs, B) !>.
   Proof with auto.
-    intros Hfree. unfold FForall. rewrite f_not_impl.
-    apply (f_exists_one_point x t(FNot A)) in Hfree. rewrite Hfree.
-    rewrite simpl_subst_not. rewrite f_not_stable...
+    induction xs... simpl. rewrite <- f_forall_and. rewrite IHxs...
   Qed.
+
+  (* A.78 *)
+  Lemma f_forall_list_impl_unused_l xs A B :
+    list_to_set xs ∩ formula_fvars A = ∅ →
+    <! ∀* xs, A ⇒ B !> ≡ <! A ⇒ (∀* xs, B) !>.
+  Proof with auto.
+    intros. induction xs as [|x xs IH]... simpl. rewrite IH; [rewrite f_forall_impl_unused_l|];
+      set_solver.
+  Qed.
+
+  Lemma f_forall_list_one_point xs ts A `{OfSameLength _ _ xs ts} :
+    NoDup xs →
+    (list_to_set xs) ∩ ⋃ (term_fvars <$> ts) = ∅ →
+    <! ∀* xs, $(AT_TermListEq (TVar <$> xs) ts) ⇒ A !> ≡ seq_subst A xs ts.
+  Proof with auto.
+    intros Hnodup Hfree. generalize dependent ts.
+    induction xs as [|x xs' IH]; simpl in *; intros.
+    - inversion H. symmetry in H1. rewrite length_zero_iff_nil in H1. subst.
+      unfold AT_TermListEq. simpl. rewrite f_true_implies...
+    - inversion H. symmetry in H1. apply length_nonzero_iff_cons in H1 as (t&ts'&?&?).
+      subst ts. rename ts' into ts. rewrite term_list_eq_cons.
+      apply NoDup_cons in Hnodup as []. rewrite <- IH by set_solver.
+      rewrite <- f_impl_curry. rewrite f_forall_list_impl_unused_l by set_solver.
+      rewrite f_forall_one_point by set_solver. f_equiv...
+  Qed.
+
   (* Fixpoint seq_subst' A xs ts : formula := *)
   (*   match xs, ts with *)
   (*   | [], [] => A *)
